\input{notes.tex}

\iftoggle{dualscreen}{\setbeameroption{show notes on second screen=right}}{}

\usepackage{gensymb}
\begin{document}

\section{Lecture 27}

\subsection{Wave Equation}
\slide[Waves travelling on strings \hfill  \hspace{2em}\begin{minipage}{0.25\textwidth}{ \includegraphics[height=1.25cm]{images/wavekids.pdf}}\end{minipage}  ]{
\vfill
\includegraphics[height=4.5cm]{images/wave_1.png}\hfill
\includegraphics[height=4.5cm]{images/wave_2.png}\hfill
\includegraphics[height=4.5cm]{images/wave_3.png}\hfill
\includegraphics[height=4.5cm]{images/wave_4.png}\hfill
\includegraphics[height=4.5cm]{images/wave_5.png}\hfill\\
\small  source: \url{https://www.youtube.com/watch?v=PVX4V5Adbzk}
\vfill
guitar strings: \url{https://vine.co/v/Oqx7BJgazKZ}
}

\slide[Wave Equation: $y_{tt}=c^2y_{xx}$]{
\uline{Plucked string under tension:} $c^2=\frac{T}{\rho}$ 
\itmz{ \item $T=$tension
\item $\rho=$mass density of the string (mass/length)}
\vfill
\centerline{\includegraphics[width=10cm]{images/sps-vibstr-tex4ht.pdf}}
\vfill
\uline{Tapped elastic rod:} $c^2=\frac{E}{\rho}$ \\
\itmz{\item $E=$Young's Modulus
\item $\rho=$mass density of the rod (mass/length)}
}

\slide[Boundary Conditions and Initial Conditions: $y_{tt}=c^2y_{xx}$]{
\centerline{\includegraphics[width=10cm]{images/sps-vibstr-tex4ht.pdf}}
Boundary Conditions:
\student{
Clamped end-points\[y(0)=y(L)=0\]}\vfill
Initial Conditions:\vfill
\student{Now we need two, because of the two time derivatives\algn{y(x,0)&=f(x)\\y_t(x,0)&=g(x)}}
\vfill
}
\subsection{Superposition}
\slide[The Wave Equation is Homogeneous: Superposition]{\vspace{-1em}
Suppose we find two solutions to the wave equation $w(x,t)$ and $z(x,t)$, then a linear combination \[y(x,t)=c_1w(x,t)+c_2z(x,t)\] is also a solution.
\vfill
Proof:
\student{
We are given 
\[ w_{tt} = c^2w_{xx}\qquad \uline{\text{and}} \qquad z_{tt} = c^2z_{xx} \]
with \[w(0)=w(L)=0 \qquad \uline{\text{and}} \qquad  z(0)=z(L)=0 \]
then 
\algn{y_{tt}&=c_1 w_{tt}+c_2z_{tt} =c_1 c^2w_{xx} + c_2 c^2 z_{xx}\\
&=c^2y_{xx}}
with 
\[y(0)=c_1w(0)+c_2z(0)=0 \qquad \uline{\text{and}} \qquad y(L)=c_1w(L)+c_2z(L)=0 \]
}
}

\slide[Decomposition into two simpler problems: Superposition]{
\centerline{ $y_{tt}=c^2y_{xx}, \quad y(0)=y(L)=0, \quad  y(x,0)=f(x), \quad y_t(x,0)=g(x)$}
\[y(x,t) = w(x,t) + z(x,t)\]
Problem 1: initial velocity, but no displacement of string
\student{\algn{w_{tt}&=c^2 w_{xx} & w(x,0)&=0  \\ w(0,t)&=w(L,t)=0&
w_t(x,0)&=g(x) \qquad \text{for } 0<x<L
}}
\vspace{.25em}

Problem 2: initial displacement, but no velocity of string
\student{\algn{z_{tt}&=c^2 z_{xx} & z(x,0)&= f(x) \qquad \text{for } 0<x<L\\z(0,t)&=z(L,t)=0 & z_t(x,0)&=0
}
\vfill
\centerline{Solve each problem by separation of variables}
}
}


\slide[Separation of Variables: Problem 1]{\vspace{-2em}
\algn{w_{tt}&=c^2 w_{xx} & w(x,0)&=0  \\ w(0,t)&=w(L,t)=0&
w_t(x,0)&=g(x) \qquad \text{for } 0<x<L
}
Try $w(x,t)=X(x)T(t)$
\student{\algn{\frac{T\pp(t)}{c^2T(t)} &= \frac{X\pp(x)}{X(x)} =-\lambda \\
\text{BCs}\Rightarrow X_n(x)&= b_n\sin\left( \frac{n\pi}{L}x\right)\\
T_n(t)&=A_n \cos\left( \frac{n\pi c}{L}t\right) + B_n \sin\left( \frac{n\pi c}{L}t\right)\\\\
w(x,0)=0 \quad \Rightarrow \quad A_n &= 0\\
\text{arbitrarily choose } B_n &= \frac{L}{n\pi c} \qquad \Rightarrow T_n\p(0) = 1 
 }
}
}

\slide[Separation of Variables + Superposition: Problem 1]{\vspace{-3em}
\algn{w_{tt}&=c^2 w_{xx} & w(x,0)&=0  \\ w(0,t)&=w(L,t)=0&
w_t(x,0)&=g(x) \qquad \text{for } 0<x<L
}
with $w_n(x,t)=\frac{L}{n\pi c} \sin\left( \frac{n\pi c}{L}t\right) b_n\sin\left( \frac{n\pi}{L}x\right) $
\student{\hfill $w(x,t) = \sum_{n=1}^\infty w_n(x,t)$ \hfill~ \algn{ \intertext{Initial condition: } w_t(x,0) &= \sum_{n=1}^\infty T_n'(0) b_n \sin\left( \frac{n\pi}{L}x\right)=\sum_{n=1}^\infty  b_n \sin\left( \frac{n\pi}{L}x\right) =  g(x)
 }\vfill
use an odd periodic extension of $g(x)$: \hfill $b_n = \frac{2}{L}\intop_0^L g(x) \sin\paren{\frac{n\pi}{L}x}$ \hfill ~
\vfill
\[w(x,t) = \sum_{n=1}^\infty \frac{L}{n\pi c} \sin\left( \frac{n\pi c}{L}t\right) b_n\sin\left( \frac{n\pi}{L}x\right) \]
}
}

\slide[Separation of Variables: Problem 2]{\vspace{-2em}
\algn{z_{tt}&=c^2 z_{xx} & z(x,0)&= f(x) \qquad \text{for } 0<x<L\\z(0,t)&=z(L,t)=0 & z_t(x,0)&=0
}
Try $z(x,t)=X(x)T(t)$
\student{\algn{\frac{T\pp(t)}{c^2T(t)} &= \frac{X\pp(x)}{X(x)} =-\lambda \\
\text{BCs}\Rightarrow X_n(x)&= c_n\sin\left( \frac{n\pi}{L}x\right)\\
T_n(t)&=A_n \cos\left( \frac{n\pi c}{L}t\right) + B_n \sin\left( \frac{n\pi c}{L}t\right)\\\\
z_t(x,0)=0 \quad \Rightarrow \quad B_n &= 0\\
\text{arbitrarily choose } A_n &=1 \qquad \Rightarrow T_n(0) = 1 
 }
}
}

\slide[Separation of Variables + Superposition: Problem 2]{\vspace{-3em}
\algn{z_{tt}&=c^2 z_{xx} & z(x,0)&= f(x) \qquad \text{for } 0<x<L\\z(0,t)&=z(L,t)=0 & z_t(x,0)&=0
}
with $z_n(x,t)= \cos\left( \frac{n\pi c}{L}t\right) c_n\sin\left( \frac{n\pi}{L}x\right) $
\student{\hfill $z(x,t) = \sum_{n=1}^\infty z_n(x,t) $ \hfill ~ \algn{\intertext{Initial condition: } z(x,0) = f(x) &= \sum_{n=1}^\infty c_n \sin\left( \frac{n\pi}{L}x\right)
 }\vfill
use an odd periodic extension of $f(x)$: $c_n = \frac{2}{L}\intop_0^L f(x) \sin\paren{\frac{n\pi}{L}x}$
\vfill
\[z(x,t) = \sum_{n=1}^\infty \cos\left( \frac{n\pi c}{L}t\right) c_n\sin\left( \frac{n\pi}{L}x\right) \]
}
}

\slide[Fourier Solution to the Wave Equation]{
\centerline{ $y_{tt}=c^2y_{xx}, \quad y(0)=y(L)=0, \quad  y(x,0)=f(x), \quad y_t(x,0)=g(x)$}
\vfill
\algn{y(x,t) &= w(x,t) + z(x,t)\\&=\sum_{n=1}^\infty \sin\left( \frac{n\pi}{L}x\right) \left[ b_n \frac{L}{n\pi c} \sin\left( \frac{n\pi c}{L}t\right)  + c_n \cos\left( \frac{n\pi c}{L}t\right)  \right] }\vfill
$c_n$ is obtained from an odd periodic extension of $f(x)$\\ \vspace{.25em}\centerline{$c_n = \frac{2}{L}\intop_0^L f(x) \sin\paren{\frac{n\pi}{L}x}$}\vfill
$b_n$ is obtained from an odd periodic extension of $g(x)$\\ \vspace{.25em}\centerline{$b_n = \frac{2}{L}\intop_0^L g(x) \sin\paren{\frac{n\pi}{L}x}$}
}
\end{document}