\input{notes.tex}

\usetikzlibrary{arrows}
\iftoggle{dualscreen}{\setbeameroption{show notes on second screen=right}}{}


\begin{document}

\section{Lecture 14}
\subsection{Preamble}


\slide[Recall: $ay''+by'+cy=f(t)\quad \text{with } y(0)=y_0, y'(0)=v_0$]{\vspace{-1em}
\[
\Rightarrow Y(s) =\underbrace{ \frac{F(s)}{as^2+bs+c}}_{\text{particular part}}+ \underbrace{\frac{ay_0s+(by_0 +av_0)}{as^2+bs+c}}_{\text{homogeneous part}}
\]

\centerline{We now focus on cases where the forcing function $f(t)$ is not continuous.}

\vfill
Two types of such forcing:\vfill
\twomini[.3]{.5}{.5}{


\student{
1. Jump Discontinuities
\subitem{Sudden change in forcing}
\vspace{1em}

\ex{Voltage jumps in a circuit.}

\vspace{1em}
\centering
\uline{Heaviside Function}}

}{

\student{2. Impulsive Forcing\subitem{Very brief and strong forcing}
\vspace{1em}
\ex{Hitting a nail with a hammer.}

\vspace{1em}
\centering
\uline{Delta Dirac Function}
}


}
\vfill
}

\subsection{The Heaviside Function}




\slide[The Heaviside Step Function: $u(t-c)$  or $H(t-c)$ or $u_c(t)$]
{\vfill
\student{Used to model effects that "turn-on" at some time $c$.}\vfill
\[u(t-c) = \begin{cases}  0 & \text{if } t< c \\ 1 & \text{if } t> c  \end{cases}\]\vfill
\centerline{\tikzplot[\xcoord{3.5}{c}\ycoord{0}{\rarray{\\0}}\ycoord{2}{1}]{1}{7}{.5}{2.5}{t}{u(t-c)}{
\draw[ultra thick, \studentcolor] (-1,0)--(3.5,0);
\draw[ultra thick, \studentcolor] (3.5,2)--(7,2);
\draw[ultra thick, dashed, \studentcolor] (3.5,0)--(3.5,2);
\draw[\studentcolor] (3.5,0) node[opendot]{};
\draw[\studentcolor] (3.5,2) node[opendot]{};
\draw[->] (4,1.6)--(3.65,1.9) node[pos=0,yshift=-1em, xshift=3em]{$\underset{t\to c^+ }{\lim}u(t-c)=1$};
\draw[->] (2.9,.4)--(3.4,.1) node[pos=0,yshift=.75em, xshift=-2.85em]{$ \underset{t\to c^- }{\lim} u(t-c)=0$};
}}
\vfill


}
\subsection{Piecewise Continuous Functions}
\slide{
\twomini[.45]{.5}{.5}{
Write the piecewise function 
\[g(t)=\begin{cases} 0 & t<1\\
-(t-2)^2+2 & 1<t<3 \\
0&t>3 \end{cases}\] in terms of the heaviside function.
}{

\tikzplot[\xcoord{3}{3}\xcoord{2}{2}\xcoord{1}{1}\ycoord{0}{\rarray{\\0}}\ycoord{1}{1}\ycoord{2}{2}]{.1}{4}{.5}{2.5}{t}{g(t)}{
\draw[ultra thick, black] (-1,0)--(1,0);
\draw[ultra thick, black] (3,0)--(7,0);
\draw[ultra thick, dashed, black] (3,0)--(3,1);
\draw[ultra thick, dashed, black] (1,0)--(1,1);
\draw[black] (3,0) node[opendot]{};
\draw[black] (3,1) node[opendot]{};
\draw[black] (1,0) node[opendot]{};
\draw[black] (1,1) node[opendot]{};
\draw[black, ultra thick, domain=1:3] plot ({\x} ,{ -(\x-2)*(\x-2)+2} );
}

}
\student{
\[g(t) =\paren{ (t-2)^2+2} \underbrace{u(t-1)}_{\carray{\text{turn on}\\\text{at $t=1$}}}\times \underbrace{(1-u(t-3))}_{\carray{\text{turn off}\\\text{at $t=3$}}}\]
or 
\[g(t) =\paren{ (t-2)^2+2}( \underbrace{u(t-1)}_{\carray{\text{turn on}\\\text{at $t=1$}}} -   \underbrace{u(t-3)}_{\carray{\text{turn off}\\\text{at $t=3$}}})\]
}
}
\subsection{Second Shift Theorem}
\slide[Laplace Tranform of the Heaviside Function]{\vspace{-1em}
\centerline{\student{\begin{tikzpicture}[xscale=2, yscale=2] \draw[] (0,0)--(0.5,0)--(0.5,0.3)--(1,0.3); \draw[] (-.15,0) node{\tiny 0}; \draw[] (-.15,0.3) node{\tiny 1}; \draw[] (0.5,.45) node{\tiny t=c};\end{tikzpicture}}}\vspace{-2em}
\student{\algn{\lap{u(t-c)}&=\lapint{u(t-c)}= \lim_{A\to c^+}\int_A^\infty e^{-st}dt\\
&\overset{s>0}{=}\lim_{A\to c^+}\frac1se^{-sA}\\
&=\boxed{e^{-sc}\frac1s}=e^{-sc}\lap{1}}
\vfill
How about the more general pattern $e^{-sc}F(s)$?}
\vfill
\uline{Second Shift Theorem}
\vfill
\student{
\[\boxed{\lap{f(t-c)u(t-c)} =e^{-sc}F(s)}\]
}
}
\slide[Proof of Second Shift Theorem]{
\algn{\lap{f(t-c)u(t-c)}&=\int_0^\infty e^{-st}\underbrace{f(t-c)u(t-c)}_{0 \text{ for } t<c}dt\\
&=\int_c^\infty e^{-st}f(t-c)dt &\arr{l}{v=t-c\\dv=dt}\\
&=\int_0^\infty e^{-s(v+c)}f(v)dv\\
&= e^{-sc}\int_0^\infty e^{-sv}f(v)dv=e^{-sc}\lap{f(t)}\\\\
\Aboxed{&\lap{f(t-c)u(t-c)} =e^{-sc}F(s) }
}
}



\slide{
\ex{Suppose $Y(s)=e^{-4s} \frac{3}{9+s^2}$, find $y(t)$.}

\student{
\algn{y(t) &=  \left[u(t) \lapinv{\frac{3}{9+s^2}} \right]_{t=t-4}\\
&= u(t-4) \left[ \sin(3t) \right]_{t=t-4}\\
&= u(t-4)  \sin(3(t-4))}

}
\vfill
\ex{Suppose $Y(s)=e^{-4s} \frac{3}{9+(s+11)^2}$, find $y(t)$.}

\student{
\algn{y(t) &=  \left[ u(t) \lapinv{\frac{3}{9+(s+11)^2}} \right]_{t=t-4}\\
&= u(t-4) \left[ e^{-11 t} \lapinv{\frac{3}{9+s^2}} \right]_{t=t-4}\\
&= u(t-4)  e^{-11(t-4)}   \sin(3(t-4))
}
}
}



\slide{
\twomini[.45]{.5}{.5}{
Write the piecewise function 
\[g(t)=\begin{cases} 0 & t<1\\
 -(t-2)^2+2 & 1<t<3 \\
0&t>3 \end{cases}\] in terms of the heaviside function.
}{

\tikzplot[\xcoord{3}{3}\xcoord{2}{2}\xcoord{1}{1}\ycoord{0}{\rarray{\\0}}\ycoord{1}{1}\ycoord{2}{2}]{.1}{4}{.5}{2.5}{t}{g(t)}{
\draw[ultra thick, black] (-1,0)--(1,0);
\draw[ultra thick, black] (3,0)--(7,0);
\draw[ultra thick, dashed, black] (3,0)--(3,1);
\draw[ultra thick, dashed, black] (1,0)--(1,1);
\draw[black] (3,0) node[opendot]{};
\draw[black] (3,1) node[opendot]{};
\draw[black] (1,0) node[opendot]{};
\draw[black] (1,1) node[opendot]{};
\draw[black, ultra thick, domain=1:3] plot ({\x} ,{ -(\x-2)*(\x-2)+2} );
}

}

\student{
\algn{g(t) &= \paren{ (t-2)^2+2} u(t-1) - \paren{ (t-2)^2+2} u(t-3)\\
&=f_1(t-1) u(t-1) + f_2(t-3) u(t-3)\\
G(s)&=e^{-s}F_1(s) - e^{-3s}F_2(s)\intertext{Need to find $f_1$ and $f_2$.  \hspace{2em}To find $f_1$, let $z_1=t-1 \;\; \Rightarrow \;\; t=z_1+1$}
f_1(t) &=-(t-2)^2 +2= -(z_1-1)^2+2\\ f_1(z_1)&=- z_1^2+2z_1+1 \quad \Rightarrow F_1(s) = -\frac{2!}{s^3}+2\frac{1!}{s^2}+\frac1{s}}
}
}


\slide{
\vfill
\student{ Let $z_2=t-3 \;\; \Rightarrow \;\; t=z_2+3$
\algn{f_2(t-3) &= -(t-2)^2 +2 =(z_2+1)^2+2\\ &=-z_2^2-2z_2+1\Rightarrow F_2(s) =-\frac{2}{s^3}-\frac{2}{s^2}+\frac1{s} \\\\
G(s)&=\left(   \frac{s^2+2s-2}{s^3}   \right)e^{-s} - \left(  \frac{s^2-2s-2}{s^3}  \right)e^{-3s}
}

}
}

\slide{\ex{$y''+y=\begin{cases}
0 & t<1\\
- (t-2)^2+2& t>1
\end{cases}$ \hspace{1.5em} with $y(0)=1, \; y'(0)=0$}
\student{\algn{ s^2Y(s)&+1Y(s)-s=\left(   \frac{s^2+2s-2}{s^3}   \right)e^{-s} \\
Y(s)&=\left(   \frac{s^2+2s-2}{(s^2+1)s^3}   \right)e^{-s} +\underbrace{\frac{s}{s^2+1}}_{\lap{\cos(t)}}\intertext{Apply partial fraction decomp....}
Y(s)&=\bigg( \underbrace{\frac{-3 s-2}{s^2+1}}_{\lap{-2\sin(t)-3\cos(t)}}+\underbrace{\frac{2}{s^2}}_{\lap{2t}}-\underbrace{\frac{2}{s^3}}_{\lap{t^2}}+\underbrace{\frac{3}{s}}_{\lap{3}}\bigg)e^{-s} +\lap{\cos(t)}\\
\\
y(t)&=u(t-1)\big[-2\sin(t-1)-3\cos(t-1)+2(t-1)\\&\qquad\qquad\quad-(t-1)^2+3\big]+\cos(t)
}
}
}
\slide{\vspace{-1.25em}
\algn{y(t)&=u(t-1)\big[-2\sin(t-1)-3\cos(t-1)+2(t-1)\\&\qquad\qquad\quad-(t-1)^2+3\big]+\cos(t)}

\vfill
\centerline{\includegraphics[width=8.5cm]{images/Heaviside_oscillator.pdf}}
}

\subsection{Impulsive Forcing}

\slide[Imagine hitting a golf ball from rest at $t=c$]{\vspace{-1em}

\tikz{\draw (0,0) node{\includegraphics[height=.175\linewidth]{images/golf_ball_1.png}}; \draw[black] (0,-.1) node[fill=white, fill opacity=0.75, text opacity=1, outer sep=0.01, inner sep=1]{\scriptsize$v(0^-)=0$}; }\hfill \tikz{\draw (0,0) node{\includegraphics[height=.175\linewidth]{images/golf_ball_2.png}}} \hfill \tikz{\draw (0,0) node{\includegraphics[height=.175\linewidth]{images/golf_ball_3.png}}; } \hfill \tikz{\draw (0,0) node{\includegraphics[height=.175\linewidth]{images/golf_ball_4.png}}; \draw[black] (.3,.1) node[fill=white, fill opacity=0.75, text opacity=1, outer sep=0.01, inner sep=1, rotate=30]{\scriptsize$v(0^+)\gg0$}; }

\tiny source:  \url{https://www.youtube.com/watch?v=6TA1s1oNpbk&t=80s}
\normalsize\vspace{-1em}

\twomini[.6]{.6}{.33}{
 \vspace{1.5em}
Suddenly a large force is applied to the ball for a very brief period of time.

\vspace{0.75em}
\student{\uline{Idea:} Describe the force as $\frac{d}{dt}u(t-c)$.

\vspace{1em}

\begin{tikzpicture}[xscale=2, yscale=2]
 \draw[] (0,0)--(0.5,0)--(0.5,0.3)--(1,0.3); 
 \draw[] (-.15,0) node{\tiny 0}; 
 \draw[] (-.15,0.3) node{\tiny 1}; 
 \draw[] (0.5,-.15) node{\tiny t=c};
 


  \draw[->] (1.1,0.00)  to [out=-30,in=-150] (1.45,0.00) node[below, xshift=-0.8em]{$ \small \frac{d}{dt}$}; 
  \draw[<-] (1.1,0.25)  to [out=30,in=150] (1.45,0.25) node[above, xshift=-0.8em]{$ \small\intop$}; 
  
  \draw[] (1.75,0)--(2.75,0); 
  \draw[->] (2.25,0)--(2.25,0.5)node[yshift=.3em]{$\infty$}; 
   \draw[] (1.6,0) node{\tiny 0}; 
 \draw[] (2.25,-.15) node{\tiny t=c};
\draw[] (3,0.35) node[align=center, draw, thin]{\footnotesize Dirac delta\\ \footnotesize function}; 
 \end{tikzpicture}

}
}{
\tikzplot[\xcoord{1}{$t=c$} ]{2}{2}{.3}{3.5}{t}{\text{force}(t)}{

\foreach \xtau in { .08}{
\draw[ultra thick] (1-\xtau,0)--(-8,0) ;
\draw[ultra thick] (1-\xtau, 0.25/\xtau)--(1+\xtau,0.25/\xtau) ;
\draw[thick, dashed] (1-\xtau,0.25/\xtau)--(1-\xtau,0) ;
\draw[thick, dashed] (1+\xtau,0.25/\xtau)--(1+\xtau,0) ;
\draw[ultra thick] (1+\xtau,0)--(6,0) ;

}
}
}\vfill
\student{\centerline{Not a well-defined function, but has a well-defined integral. }}
}



\subsection{Dirac Delta}


\slide[Delta Dirac Function: $\delta(t-c) =\frac{d}{dt} u(t-c)$]{\vspace{-0.75em}
\textbf{Theorem:} For any function $f(t)$ that is integrable in some neighbourhood around $c$\[\int_{-\infty}^{\infty} \delta(t-c) f(t) dt = f(c)\]
Integrating a function $f(t)$ against $\delta(t-c)$ essentially "selects" the value of  $f(t)$ at $t=c$
\vfill

More generally
\twomini[.25]{.65}{.35}{
\[\int_a^b \delta(t-c)f(t) dt =\student{ \begin{cases} f(c)& a\leq c\leq b  \\ 0&\text{otherwise}\end{cases}}\]
}{


\tikzplot[\xcoord{0.8}{c}\xcoord{-0.5}{a}, \xcoord{1.5}{b} ]{1.8}{2.2}{.7}{2}{t}{}{

\foreach \xtau in { .01}{
\draw[ultra thick] (0.8-\xtau,0)--(-8,0) ;
\draw[ultra thick] (0.8-\xtau, 0.3/\xtau)--(1+\xtau,0.3/\xtau) ;
\draw[] (0.8-\xtau,0.25/\xtau)--(0.8-\xtau,0) ;
\draw[] (0.8+\xtau,0.25/\xtau)--(0.8+\xtau,0) ;
\draw[] (1.55,1.7) node{$\delta(t-c)$};
\draw[ultra thick] (0.8+\xtau,0)--(6,0) ;
\draw[black, ultra thick, domain=-2:2.2] plot (\x,0.9*\x^2-0.45*\x^3) node[right, above, xshift=-1em, yshift=2em]{$f(t)$};

}
}


}
}

\slide[Sketch of ``proof'':]{
Approximate the Dirac delta function as normalized pulse:\[ \text{Let }\delta_\tau =  \frac{u(t+\tau)-u(t-\tau)}{2\tau}, \text{and use the approximation  }\delta(t)\approx \lim_{\tau \to 0} \delta_\tau(t)\]
\algn{\int_{-\infty}^{\infty}\delta(t-c)f(t) dt &= \int_{-\infty}^{\infty} \left( \lim_{\tau \to 0} \delta_{\tau}(t-c)\right) f(t) dt\\
&=\lim_{\tau \to 0}  \int_{-\infty}^{\infty}  \delta_{\tau}(t-c) f(t) dt\\
&=\lim_{\tau \to 0}  \frac{1}{2\tau}\int_{c-\tau}^{c+\tau}f(t)dt\\&=\lim_{\tau \to 0} \frac{F(c+\tau)-F(c-\tau)}{2\tau} =f(c)
}
}

\slide[Laplace transform of $\delta(t)$]{
Integrating a function $f(t)$ against $\delta(t-c)$ essentially "selects" the value of  $f(t)$ at $t=c$\vfill
Assuming $c>0$
\student{
\algn{\ucover{\lap{\delta(t-c)}=} & \lapint{\delta(t-c) }\\
=&\int_{-\infty}^{\infty} e^{-st} \delta(t-c) dt =e^{-sc}}
}
Special case: $c=0$
\student{\algn{\ucover{\lap{\delta(t)}=\lim_{c \to 0^+}  \lap{\delta(t-c)}} =  \lim_{c \to 0^+}  e^{-sc} = 1 }}

}
\subsection{Example}

\slide[Solve: \hfill $y\pp+6y\p+45y=6\delta(t-5)$ \hfill with $\larray{y(0)=1\\y\p(0)=0}$]{\vspace{-2em}\student{
\algn{
 (s^2+6s+45)Y(s)-(6+s)&= 6e^{-5s} \quad \Rightarrow \quad Y(s) =\frac{6e^{-5s}+s+6}{s^2+6s+45} \\\\
 Y(s)= e^{-5s}\underbrace{\frac{6}{(s+3)^2+36}}_{\lap{e^{-3t}\sin(6t)}} &+ \underbrace{\frac{s+3}{(s+3)^2+36}}_{\lap{e^{-3t}\cos(6t)}} + \frac{3}{(s+3)^2+36} \\\\
y(t) = \left[ e^{-3t}\sin(6t)\right]_{t=t-5} &+ e^{-3t}\paren{\cos(6t) + \frac12 \sin(6t) }\\
= e^{-3(t-5)}\sin(6(t-5)) &+  e^{-3t}\paren{\cos(6t) + \frac12 \sin(6t) }
}  
}
}

\slide[]{
\[y(t)=e^{-3(t-5)}\sin(6(t-5)) +  e^{-3t}\paren{\cos(6t) + \frac12 \sin(6t) }\]
\vfill
\centerline{\includegraphics[width=8.5cm]{images/Dirac_overdamped.pdf}}
}


\begin{comment}
\subsection{Convolution Theorem}
\slide[Products in Laplace Space]{\vspace{-1em}
The second shift theorem is a special case of a product in Laplace space\[\lap{f(t-c)u(t-c)} = \underbrace{e^{-sc}}_{G(s)}F(s)\]\vfill
Inversion of the general case requires the use of a convolution
\[\lapinv{F(s) G(s) } = (f * g)(t) = \intop_0^t f(\tau)g(t-\tau) d\tau\] 
\ex{$\lapinv{\frac{e^{-3s}}{s} \frac{2}{s^2} }$ \student{Note:  $\lapinv{e^{-3s}\frac{2}{s^3}}=u(t-3)(t-3)^2$}}
\student{\algn{&=\intop_0^t u(\tau-3) 2(t-\tau) d \tau =\begin{cases} 0&t<3 \\ \intop_3^t 2(t-\tau) d \tau  & t>3 \end{cases} \\
&=\begin{cases} 0&t<3 \\  \left[2t\tau-\tau^2\right]_{\tau=3}^{t} & t>3 \end{cases}  =  u(t-3) (t-3)^2
}}
}
\slide{\ex{$y\p+6y=u(t-1)\student{=\begin{cases}
0 & t<1\\
1 & t\geq1
\end{cases}}$ \hspace{1.5em} with $\larray{y(0)=y_0\\y'(0)=v_0}$}
\student{\twomini[.55]{.6}{.3}{\algn{ sY-&y_0+6Y=\frac{e^{-s}}{s}\\
Y&=\frac{\frac{e^{-s}}{s}+y_0}{s+6}=\frac{e^{-s}}{s(s+6)}+\frac{y_0}{s+6}\\
Y(s)&=\frac{1}{6}\frac{e^{-s}}{s}-\frac{1}{6}\frac{e^{-s}}{s+6}+\frac{y_0}{s+6}\\
& \downarrow \mathcal{L}^{-1}\\
y(t)&=\frac16 u(t-1)-\frac16 e^{-6(t-1)} u(t-1)+y_0e^{-6t}
}\vfill}{$\frac{1}{s(s+6)}=\frac{A}{s}+\frac{B}{s+6}$\\~\\$\Rightarrow 1=A(s+6)+Bs $\\~\\$\Rightarrow \arr{l}{1=6A\\0=A+B}$ \\~\\$\Rightarrow \arr{l}{A=\frac16\\B=-\frac16}$ \vfill}}
\tikzplot[
\student{\xcoord{3}{1} \ycoord{1.25}{\frac16}}
]{.1}{10}{.1}{1.5}{t}{y(t)}{
\student{
\draw[domain=0:2, thick, samples=100] plot ({\x*1.5}, {.8*exp(-\x)});
\draw[domain=2:10, thick, samples=100] plot ({\x*1.5}, {.8*exp(-\x)+(1-exp(-(\x-2)))*1.25});
\draw[domain=0:10, thick, dashed, samples=100] plot ({\x*1.5}, {1.25});
}}
}



\slide{\ex{$y\pp+2y\p+5y=u(t-5)-u(t-15)$, \quad $y(0)=0.1$, $y\p(0)=0$}
\student{
\algn{s^2Y(s)-&0.1s+2sY(s)-0.2+5Y(s)=\frac{e^{-5s}}{s} - \frac{e^{-15s}}{s}\\
Y(s)&= \frac{  \paren{\frac{e^{-s}}{s} - \frac{e^{-2s}}{s}} + 0.1s+0.2}{s^2+2s+5}\\
&=  \paren{ e^{-5s} - e^{-15s}}  \underbrace{\frac{ 1}{s(s^2+2s+5)}}_{F(s)}+   \underbrace{\frac{ 0.1s +0.2}{s^2+2s+5}}_{\text{homogeneous part}}\\
s^2+2s+5 &= (s+1)^2+4 \Rightarrow\text{homog. part} = \underbrace{\frac{0.1s}{ (s+1)^2+4}}_{\text{exp} \cdot \cos}  + \underbrace{\frac{0.2}{ (s+1)^2+4}}_{\text{exp} \cdot \sin}
\\\\
y(t)&=u(t-5)\left[ \lapinv{F(s)} \right]_{t=t-5}\\
&\phantom{=} - u(t-15)\left[ \lapinv{F(s)} \right]_{t=t-15}\\
&\phantom{=} + 0.1e^{-t}\cos(2t)+0.1 e^{-t}\sin(2t)
}
}
}%end slide

\settoggle{covered}{false}
\slide{$\lapinv{\frac{1}{s(s^2+2s+5)}}=\;???$ 

\student{
\algn{F(s)=\frac{1}{s(s^2+2s+5)} & = \frac{A}{s} +\frac{Bs+C}{s^2+2s+5}\\
1&=As^2+2As+5A + Bs^2+Cs\\
\text{constant terms: } 1&= 5A \qquad \Rightarrow A=\frac15 \\
\text{$s$ terms: } 0 &= 2A+C   \qquad \Rightarrow C=-2A=-\frac25\\
\text{$s^2$ terms: } 0 &=	A+B  \qquad \Rightarrow B=-A=-\frac15\\
F(s) &= \frac{1}{5s} - \frac15 \frac{s+2}{(s+1)^2+2^2}\\
&=  \frac{1}{5s} -  \frac15 \paren{\frac{s+1}{(s+1)^2+2^2}  - \frac{1}{(s+1)^2+2^2}}  \\
f(t) &= \frac15 \paren{1-e^{-t}\paren{cos(2t) -\frac12 \sin(2t)}}}
}
}

\slide{\vspace{-2em}
\algn{y(t)&=u(t-5)\frac15 \paren{1-e^{-(t-5)}\paren{cos(2(t-5)) -\frac12 \sin(2(t-5))}}\\
&\phantom{=} - u(t-15)\frac15 \paren{1-e^{-(t-15)}\paren{cos(2(t-15)) -\frac12 \sin(2(t-15))}}\\\
&\phantom{=} + 0.1e^{-t}(\cos(2t)+\sin(2t))}

\vspace{1em}
\centerline{\includegraphics[width=8.5cm]{images/Heaviside_jiggle.pdf}}
}
\end{comment}

\end{document}